feat(jmpIEpcc): finishing implementation IEpcc

theories/ftlr/JmpIEpcc.v
@@ -21,45 +21,33 @@ Section fundamental.
 
   (* Mask after the jump, depending on the address of the pc and the address
    of a *)
-  Definition allow_jmp_mask (pc_a a : Addr) : coPset
+  Definition allow_jmp_mask (pc_a b : Addr) : coPset
     :=
-    if decide (pc_a = a)
+    if decide (pc_a = b)
     then (⊤ ∖ ↑logN.@pc_a)
-    else(⊤ ∖ ↑logN.@pc_a ∖ ↑logN.@a).
+    else(⊤ ∖ ↑logN.@pc_a ∖ ↑logN.@b).
 
   Definition allow_jmp_mask_reg (cond : Prop) `{Decision cond}
     (regs : Reg) (r : RegName) (pc_a : Addr)
     (p : Perm) (b e a : Addr) : coPset :=
-    if decide (reg_allows_IEpcc_jmp regs r p b e a /\ cond /\ pc_a ≠ b)
+    if decide (reg_allows_IEpcc_jmp regs r p b e a /\ cond)
     then allow_jmp_mask pc_a b
     else (⊤ ∖ ↑logN.@pc_a).
 
-  (* The necessary resources to close the region again,
-     except for the points to predicate, which we will store separately *)
-  (* Definition region_open_resources2 *)
-  (*   (pc_a : Addr) (a : Addr) *)
-  (*   (w1 : Word) (w2 : Word) *)
-  (*   (P1 P2 : D) *)
-  (*   : iProp Σ := *)
-  (*   ▷ P1 w1 *)
-  (*   ∗ persistent_cond P1 *)
-  (*   ∗ ((▷ ∃ w1, a ↦ₐ w1 ∗ P1 w1) *)
-  (*      ={allow_jmp_mask pc_a a, ⊤ ∖ ↑logN.@pc_a}=∗ emp)%I. *)
-
   Definition region_open_resources
-    (pc_a : Addr) (a : Addr) (w : Word) (P : D) : iProp Σ :=
+    (pc_a : Addr) (b : Addr) (w : Word) (P : D) : iProp Σ :=
     (▷ P w
        ∗ persistent_cond P
-       ∗ ((▷ ∃ w, a ↦ₐ w ∗ P w)
-        ={allow_jmp_mask pc_a a, ⊤ ∖ ↑logN.@pc_a}=∗ emp))%I.
+       ∗ ((▷ ∃ w, b ↦ₐ w ∗ P w)
+        ={allow_jmp_mask pc_a b, ⊤ ∖ ↑logN.@pc_a}=∗ emp))%I.
 
   Definition allow_jmp_res_mem
-    (pc_a : Addr) (a : Addr)
+    (pc_a : Addr) (b : Addr)
     (P : D): iProp Σ :=
-    (|={⊤ ∖ ↑logN.@pc_a, allow_jmp_mask pc_a a}=>
-       (if decide (pc_a = a)
+    (|={⊤ ∖ ↑logN.@pc_a, allow_jmp_mask pc_a b}=>
+       (if decide (pc_a = b)
         then True
-        else ∃ w, a ↦ₐ w ∗ region_open_resources pc_a a w P)
+        else ∃ w, b ↦ₐ w ∗ region_open_resources pc_a b w P)
     )%I.
 
   (* Description of what the resources are supposed to look like after opening the
@@ -67,11 +55,11 @@ Section fundamental.
   Definition allow_jmp_res (cond : Prop) `{Decision cond} (regs : Reg) (r : RegName)
     (pc_a : Addr) (p : Perm) (b e a : Addr)
     (P : D): iProp Σ :=
-    (if decide (reg_allows_IEpcc_jmp regs r p b e a /\ cond /\ pc_a ≠ b)
-       then
-         (∀ w1 regs', ▷ □ (P w1 -∗ (interp_expr_gen interp regs' w1 (WCap RW b e a))))
-           ∗ allow_jmp_res_mem pc_a b P
-       else True)%I.
+    (if decide (reg_allows_IEpcc_jmp regs r p b e a /\ cond)
+     then
+       (∀ w1 regs', ▷ □ (P w1 -∗ (interp_expr_gen interp regs' w1 (WCap RW b e a))))
+       ∗ allow_jmp_res_mem pc_a b P
+     else True)%I.
 
   Lemma create_jmp_res (cond : Prop) `{Decision cond}:
     ∀ (regs : leibnizO Reg) (r : RegName)
@@ -111,28 +99,19 @@ Section fundamental.
       rewrite /region_open_resources /allow_jmp_mask decide_False //=.
       iFrame "∗ #".
       by iModIntro.
-      (* iIntros "Ha". *)
-      (* iDestruct "Ha" as (w1' w2') "(Hw1' & HP1' & Hw2' & HP2')". *)
-      (* iMod ("Hcls_a'" with "[Hw2' HP2']") as "_"; first (iExists _ ; iFrame). *)
-      (* iMod ("Hcls_a" with "[Hw1' HP1']") as "_"; first (iExists _ ; iFrame). *)
-      (* done. *)
   Qed.
 
-  (* Definition allow_jmp_mem_res *)
-  (*   (mem : Mem) (pc_a : Addr) (pc_w : Word) (a : Addr) (P : D) := *)
-  (*   (if decide (pc_a = a) *)
-  (*   then ∃ w2, ⌜mem = (<[pc_a:=pc_w]> ∅)⌝ ∗ region_open_resources pc_a a w P *)
-  (*   else *)
-  (*     if decide (pc_a = (a^+1)%a) *)
-  (*     then ∃ w1, ⌜mem = <[a:=w1]> (<[pc_a:=pc_w]> ∅)⌝ ∗ region_open_resources pc_a a (a^+1)%a w1 P1 *)
-  (*     else ∃ w1 w2, *)
-  (*         ⌜mem = <[(a^+1)%a:=w2]> (<[a:=w1]> (<[pc_a:=pc_w]> ∅))⌝ ∗ region_open_resources2 pc_a a (a^+1)%a w1 w2 P1 P2)%I. *)
+  Definition allow_jmp_mem_res
+    (mem : Mem) (pc_a : Addr) (pc_w : Word) (b : Addr) (P : D) :=
+    (if decide (pc_a ≠ b)
+     then ∃ w, ⌜mem = <[b:=w]> (<[pc_a:=pc_w]> ∅)⌝ ∗ region_open_resources pc_a b w P
+     else ⌜mem = <[pc_a:=pc_w]> ∅⌝)%I.
 
   Definition allow_jmp_mem (cond : Prop) `{Decision cond}
     (regs : Reg) (mem : Mem) (r : RegName)
     (pc_a : Addr) (pc_w : Word) (p : Perm) (b e a : Addr) (P : D) :=
-    (if decide (reg_allows_IEpcc_jmp regs r p b e a /\ cond /\ pc_a ≠ b)
-     then ∃ w, ⌜mem = <[b:=w]> (<[pc_a:=pc_w]> ∅)⌝ ∗ region_open_resources pc_a b w P
+    (if decide (reg_allows_IEpcc_jmp regs r p b e a /\ cond)
+     then allow_jmp_mem_res mem pc_a pc_w b P
      else ⌜mem = <[pc_a:=pc_w]> ∅⌝)%I.
 
   Lemma jmp_res_implies_mem_map (cond : Prop) `{Decision cond}:
@@ -159,115 +138,91 @@ Section fundamental.
       + rewrite /allow_jmp_mem decide_False //=.
       + iModIntro. iNext. by iApply memMap_resource_1.
     }
-    destruct Hdec as ((Hreg & -> & Hwb) & Hcond & Hb).
+    destruct Hdec as ((Hreg & -> & Hwb) & Hcond).
     iDestruct "HJmpRes" as "[Hexec HJmpRes]".
     iMod "HJmpRes" as "HJmpRes".
-    rewrite /allow_jmp_mask /allow_jmp_mem.
-    repeat (rewrite decide_False;[|done]).
+    rewrite /allow_jmp_mask /allow_jmp_mem /allow_jmp_mem_res.
+
+    case_decide as Hb ; simplify_eq.
+    { (* pc_a = b *)
+      iExists _.
+      iModIntro.
+      rewrite decide_True; [|by rewrite /reg_allows_IEpcc_jmp].
+      rewrite decide_False //=; last (by intro).
+      iSplitR "Hpc_a"; eauto.
+      iNext.
+      rewrite memMap_resource_1; auto; iFrame.
+    }
 
     iDestruct "HJmpRes" as (w) "(Ha & HJmpRest)".
     iModIntro.
     iExists (<[b:=w]> (<[pc_a:=pc_w]> ∅)).
-    rewrite decide_True;[|done].
+    repeat (rewrite decide_True;[|done]).
     iSplitL "HJmpRest"; eauto.
     rewrite memMap_resource_2ne; auto; iFrame.
   Qed.
 
   (* Close the invariants, in case of fail*)
-  (* Lemma mem_map_recover_res *)
-  (*   (cond : Por(mem : Mem) (pc_a a : Addr) (pc_w : Word) (P : D): *)
-  (*   allow_jmp_mem mem pc_a pc_w a P *)
-  (*   -∗ ([∗ map] a'↦w' ∈ mem, a' ↦ₐ w') *)
-  (*   ={allow_jmp_mask pc_a a , ⊤ ∖ ↑logN.@pc_a}=∗ pc_a ↦ₐ pc_w. *)
-  (* Proof. *)
-  (*   iIntros (Hneq) "HJmpMem Hmem". *)
+  Lemma mem_map_recover_res
+    (mem : Mem) (pc_a b : Addr) (pc_w : Word) (P : D):
+    allow_jmp_mem_res mem pc_a pc_w b P
+    -∗ ([∗ map] a'↦w' ∈ mem, a' ↦ₐ w')
+    ={allow_jmp_mask pc_a b , ⊤ ∖ ↑logN.@pc_a}=∗ pc_a ↦ₐ pc_w.
+  Proof.
+    iIntros "HJmpMem Hmem".
 
-  (*   rewrite /allow_jmp_mem_res /allow_jmp_mask. *)
-  (*   case_decide as Ha; simplify_eq. *)
-  (*   { (* pc_a = a *) *)
-  (*     iDestruct "HJmpMem" as (w2) "(->&Hres)". rewrite /region_open_resources. *)
-  (*     rewrite memMap_resource_2ne; auto. *)
-  (*     iDestruct "Hmem" as "(Ha0' & Ha0)". *)
-  (*     iDestruct "Hres" as "(HP2 & _ & Hcls')". *)
-  (*     rewrite /allow_jmp_mask. *)
-  (*     rewrite decide_False //= decide_True //=. *)
-  (*     iMod ("Hcls'" with "[HP2 Ha0']") as "_" ; [iNext ; iExists w2; iFrame|auto]. *)
-  (*   } *)
+    rewrite /allow_jmp_mem_res /allow_jmp_mask.
+    case_decide as Hb; simplify_eq.
+    { (* pc_a ≠ b *)
+      rewrite decide_False ; last done.
+      iDestruct "HJmpMem" as (w) "(->&Hres)". rewrite /region_open_resources.
+      rewrite memMap_resource_2ne; auto.
+      iDestruct "Hmem" as "(Hb & Hpc_a)".
+      iDestruct "Hres" as "(HP & _ & Hcls)".
+      rewrite /allow_jmp_mask.
+      rewrite decide_False //=.
+      iMod ("Hcls" with "[HP Hb]") as "_"; [iNext ; iExists w; iFrame|auto].
+    }
 
-  (*   case_decide as Ha'; simplify_eq. *)
-  (*   { (* pc_a = a+1 *) *)
-  (*     iDestruct "HJmpMem" as (w1) "(->&Hres)". rewrite /region_open_resources. *)
-  (*     rewrite memMap_resource_2ne; auto. *)
-  (*     iDestruct "Hmem" as "(Ha0 & Ha0')". *)
-  (*     iDestruct "Hres" as "(HP1 & _ & Hcls')". *)
-  (*     rewrite /allow_jmp_mask. *)
-  (*     rewrite decide_False //= decide_True //=. *)
-  (*     iMod ("Hcls'" with "[HP1 Ha0]") as "_" ; [iNext ; iExists w1; iFrame|auto]. *)
-  (*   } *)
-
-  (*   (* a ≠ a0 ∧ a ≠ a0+1 *) *)
-  (*   iDestruct "HJmpMem" as (w1 w2) "(->&Hres)". rewrite /region_open_resources2. *)
-  (*   rewrite memMap_resource_3ne; auto. *)
-  (*   iDestruct "Hmem" as "(Ha0' & Ha0 & Ha)". *)
-  (*   iDestruct "Hres" as "(HP1 & HP2 & _& _ & Hcls')". *)
-  (*   rewrite /allow_jmp_mask. *)
-  (*   rewrite decide_False //= decide_False //=. *)
-  (*   iMod ("Hcls'" with "[HP1 HP2 Ha0 Ha0']") as "_"; [iNext ; iExists w1,w2; iFrame|auto]. *)
-  (* Qed. *)
+    (* pc_a = b  *)
+    rewrite decide_True ; last done.
+    iDestruct "HJmpMem" as "->".
+    rewrite memMap_resource_1; auto.
+  Qed.
 
   (* Close the invariants, in case of jump to IEpair *)
-  (* Lemma mem_map_recover_res_ie *)
-  (*   (mem : Mem) (pc_a a : Addr) (pc_w wpc widc : Word) (P P1 P2 : D): *)
-  (*   (a ^+ 1)%a ≠ a -> *)
-  (*   mem !! a = Some wpc -> *)
-  (*   mem !! (a ^+ 1)%a = Some widc -> *)
+  Lemma mem_map_recover_res_ie
+    (mem : Mem) (pc_a b : Addr) (pc_w wpc : Word) (P P1 : D):
+    mem !! b = Some wpc ->
 
-  (*   allow_jmp_mem_res mem pc_a pc_w a P1 P2 *)
-  (*   -∗ ([∗ map] a'↦w' ∈ mem, a' ↦ₐ w') *)
-  (*   ={allow_jmp_mask pc_a a (a ^+1)%a, ⊤ ∖ ↑logN.@pc_a}=∗ *)
-  (*     if (decide (pc_a = a)) *)
-  (*     then pc_a ↦ₐ pc_w ∗ ⌜pc_w = wpc ⌝ *)
-  (*     else *)
-  (*       if (decide (pc_a = (a^+1)%a)) *)
-  (*       then pc_a ↦ₐ widc ∗ ⌜pc_w = widc⌝ ∗ ▷ P1 wpc ∗ persistent_cond P1 *)
-  (*       else pc_a ↦ₐ pc_w ∗ ▷ P1 wpc ∗ ▷ P2 widc ∗ persistent_cond P1 ∗ persistent_cond P2. *)
-  (* Proof. *)
-  (*   iIntros (Hneq Hmem_a Hmem_a') "HJmpMem Hmem". *)
-  (*   rewrite /allow_jmp_mem_res /allow_jmp_mask. *)
+    allow_jmp_mem_res mem pc_a pc_w b P1
+    -∗ ([∗ map] a'↦w' ∈ mem, a' ↦ₐ w')
+    ={allow_jmp_mask pc_a b, ⊤ ∖ ↑logN.@pc_a}=∗
+    if (decide (pc_a = b))
+    then pc_a ↦ₐ pc_w ∗ ⌜pc_w = wpc ⌝
+    else pc_a ↦ₐ pc_w ∗ ▷ P1 wpc ∗ persistent_cond P1.
+  Proof.
+    iIntros (Hmem_b) "HJmpMem Hmem".
+    rewrite /allow_jmp_mem_res /allow_jmp_mask.
 
-  (*   case_decide as Ha; simplify_eq. *)
-  (*   { (* a = a0 *) *)
-  (*     iDestruct "HJmpMem" as (w2) "(->& HP2& %Hpers2& Hcls')". *)
-  (*     rewrite /allow_jmp_mask. *)
-  (*     rewrite decide_False //= decide_True //=. *)
-  (*     rewrite memMap_resource_2ne; auto. *)
-  (*     simplify_map_eq. *)
-  (*     iDestruct "Hmem" as  "[Ha0' Ha0]". *)
-  (*     iMod ("Hcls'" with "[HP2 Ha0']") as "_" ; [iNext;iExists widc;iFrame "∗ #"|auto]. *)
-  (*   } *)
-
-  (*   case_decide as Ha'; simplify_eq. *)
-  (*   { (* a = a0+1 *) *)
-  (*     iDestruct "HJmpMem" as (w1) "(->& HP1& %Hpers1& Hcls')". *)
-  (*     iDestruct "HP1" as "#HP1". *)
-  (*     rewrite /allow_jmp_mask. *)
-  (*     rewrite decide_False //= decide_True //=. *)
-  (*     rewrite memMap_resource_2ne; auto. *)
-  (*     simplify_map_eq. *)
-  (*     iDestruct "Hmem" as "[Ha0' Ha0]". *)
-  (*     iMod ("Hcls'" with "[HP1 Ha0']") as "_" ; [iNext;iExists wpc;iFrame "∗ #"|auto]. *)
-  (*   } *)
-
-  (*   (* a ≠ a0 ∧ a ≠ a0+1 *) *)
-  (*   iDestruct "HJmpMem" as (w1 w2) "(->& HP1& HP2& %Hpers1& %Hpers2& Hcls')". *)
-  (*   rewrite /region_open_resources2. *)
-  (*   iDestruct "HP1" as "#HP1"; iDestruct "HP2" as "#HP2". *)
-  (*   rewrite /allow_jmp_mask; case_decide ; simplify_eq; case_decide ; simplify_eq. *)
-  (*   rewrite memMap_resource_3ne; auto. *)
-  (*   simplify_map_eq. *)
-  (*   iDestruct "Hmem" as  "(Ha0' & Ha0 & Ha)". *)
-  (*   iMod ("Hcls'" with "[HP1 HP2 Ha0' Ha0]") as "_"; [iNext;iExists wpc,widc;iFrame "∗ #"|auto]. *)
-  (* Qed. *)
+    case_decide as Hb; simplify_eq
+    ; [ rewrite decide_False //= | rewrite decide_True //= ]
+    ; [ rewrite decide_False //= | rewrite decide_True //= ]
+    ; cycle 1.
+    { (* pc_a = b *)
+      iDestruct "HJmpMem" as "->".
+      simplify_map_eq.
+      rewrite memMap_resource_1; auto.
+    }
+    (* pc_a ≠ b *)
+    iDestruct "HJmpMem" as (w) "(->& HP& %Hpers& Hcls)".
+    iDestruct "HP" as "#HP".
+    rewrite /allow_jmp_mask; case_decide ; simplify_eq.
+    rewrite memMap_resource_2ne; auto.
+    simplify_map_eq.
+    iDestruct "Hmem" as "[Hb Hpc_a]".
+    iMod ("Hcls" with "[HP Hb]") as "_" ; [iNext;iExists wpc ; iFrame "∗ #"|auto].
+  Qed.
 
   (* Derice pure conds =allow_jmp_mmap_or_true= from =cond_jmp= *)
   Lemma mem_map_implies_pure_conds:
@@ -279,18 +234,28 @@ Section fundamental.
       -∗ ⌜mem !! pc_a = Some pc_w⌝ ∗ ⌜allow_jmp_mmap_or_true cond_jmp r regs mem⌝.
   Proof.
     iIntros (regs mem r pc_a pc_w p b e a P Hrinr) "HJmpMem".
-    rewrite /allow_jmp_mem.
+    rewrite /allow_jmp_mem /allow_jmp_mem_res.
     case_decide as Hdec ; cycle 1.
     { iDestruct "HJmpMem" as "->".
       iSplitR. by rewrite lookup_insert.
       iExists p,b,e,a.
       iSplitR; auto.
-      (* rewrite decide_False //=. *)
-      admit.
+      rewrite decide_False //=.
     }
-    destruct Hdec as ((Hreg & -> & Hwb) & Hcond & Hb).
+    destruct Hdec as ((Hreg & -> & Hwb) & Hcond).
 
-    (* pc_a ≠ a ∧ pc_a ≠ a+1 *)
+    case_decide as Hb; simplify_eq ; cycle 1.
+    { (* pc_a ≠ b *)
+      iDestruct "HJmpMem" as "->".
+      iSplitL.
+      by iPureIntro; simplify_map_eq.
+      iExists IEpcc,b,e,a.
+      iSplitR; auto.
+      case_decide; auto.
+      iExists pc_w.
+      by iPureIntro ; simplify_map_eq.
+    }
+    (* pc_a = b *)
     iDestruct "HJmpMem" as (w) "[%Hmem _]" ; subst.
     iSplitL.
     by iPureIntro; simplify_map_eq.
@@ -299,9 +264,9 @@ Section fundamental.
     case_decide; auto.
     iExists w.
     by iPureIntro ; simplify_map_eq.
-  Admitted.
+  Qed.
 
-  Lemma jmpiepair_case (regs : leibnizO Reg) (p : Perm)
+  Lemma jmpiepcc_case (regs : leibnizO Reg) (p : Perm)
         (b e a : Addr) (widc w : Word) (src : RegName) (P : D):
     ftlr_instr regs p b e a widc w (JmpIEpcc src) P.
   Proof.
@@ -396,15 +361,14 @@ Section fundamental.
       rewrite !decide_True //=.
 
       (* Step 4: return all the resources we had *)
-      iMod ((mem_map_recover_res_ie _ _ _ w wpc widc0 P P1 P2) with "HJmpMem Hmem") as "Ha"
+      iMod ((mem_map_recover_res_ie _ _ _ w wpc P P1) with "HJmpMem Hmem") as "Hb"
       ; auto; iModIntro.
 
-      case_decide as Ha0; simplify_eq.
-      { (* a = a0 *)
+      case_decide as Hb0; simplify_eq.
+      { (* a = b0 *)
+        iDestruct "Hb" as "[Hb ->]".
 
-        iDestruct "Ha" as "[Ha0 ->]".
-
-        iMod ("Hcls" with "[HP Ha0]") as "_"; [iNext;iExists wpc;iFrame|iModIntro].
+        iMod ("Hcls" with "[HP Hb]") as "_"; [iNext;iExists wpc;iFrame|iModIntro].
         iApply wp_pure_step_later; auto.
         iNext ; iIntros "_".
         destruct wpc; cbn in Hi; try done.
@@ -414,25 +378,10 @@ Section fundamental.
         iPureIntro; apply regmap_full_dom in Hsome; rewrite -Hsome; set_solver.
       }
 
-      case_decide as Ha0'; simplify_eq.
-      { (* a = a0+1 *)
-
-        iDestruct "Ha" as "(Ha0 & -> & HP1 & %Hpers1)".
-        iDestruct "HP1" as "#HP1".
-
-        iMod ("Hcls" with "[HP Ha0]") as "_"; [iNext;iExists widc0;iFrame|iModIntro].
-        iApply wp_pure_step_later; auto.
-        iNext ; iIntros "_".
-        iApply ("Hexec" $! _ widc0) ; iFrame "∗ #".
-        iRight; destruct widc0; cbn in Hi; try done.
-        rewrite insert_commute //=.
-        repeat (iSplit ; try done).
-      }
-
-      (* a ≠ a0 ∧ a ≠ a0+1 *)
-      iDestruct "Ha" as "(Ha & HP1 & HP2 & %Hpers1 & %Hpers2)".
-      iDestruct "HP1" as "#HP1"; iDestruct "HP2" as "#HP2".
-      iMod ("Hcls" with "[HP Ha]") as "_"; [iNext;iExists w;iFrame|iModIntro].
+      (* pc_a ≠ b0 *)
+      iDestruct "Hb" as "(Hb & HP1 & %Hpers1)".
+      iDestruct "HP1" as "#HP1".
+      iMod ("Hcls" with "[HP Hb]") as "_"; [iNext;iExists w;iFrame|iModIntro].
       iApply wp_pure_step_later; auto.
       iNext; iIntros "_".
       iApply "Hexec" ; iFrame "∗ #".
@@ -441,7 +390,7 @@ Section fundamental.
 
     - (* fail *)
       rewrite /allow_jmp_mask_reg /allow_jmp_mem /allow_jmp_res.
-      destruct (decide ((reg_allows_IEpair_jmp
+      destruct (decide ((reg_allows_IEpcc_jmp
                           (<[PC:=WCap p b e a]> (<[idc:=widc]> regs))
                           src p0 b0 e0 a0) /\ cond_jmp)) as [HallowJmp|_]
       ; cycle 1.
@@ -454,15 +403,11 @@ Section fundamental.
         iApply wp_value; auto; iIntros; discriminate.
       }
 
-      assert ((a0 ^+ 1)%a ≠ a0) as Ha0eq
-      by (destruct HallowJmp as
-           [(_ & _ & Hwb%Is_true_true_1%withinBounds_true_iff & _) _]; solve_addr).
-
       (* Step 4: return all the resources we had *)
-      iMod (mem_map_recover_res with "HJmpMem Hmem") as "Ha"; auto.
+      iMod (mem_map_recover_res with "HJmpMem Hmem") as "Hb"; auto.
 
       iModIntro.
-      iMod ("Hcls" with "[Ha HP]") as "_";[iExists w;iFrame|iModIntro].
+      iMod ("Hcls" with "[Hb HP]") as "_";[iExists w;iFrame|iModIntro].
       iApply wp_pure_step_later; auto.
       iNext; iIntros "_".
       iApply wp_value; auto; iIntros; discriminate.
